src/tools/lifter/bir_lifting_machinesLib.sml
@@ -11,7 +11,7 @@ open bir_exp_liftingLib bir_lifting_machinesTheory
 
 val ERR = mk_HOL_ERR "bir_lifting_machinesLib"
 val wrap_exn = Feedback.wrap_exn "bir_lifting_machinesLib"
-
+fun mkselnm ty f = TypeBasePure.mk_recordtype_fieldsel{tyname=ty,fieldname=f}
 fun syntax_fns n d m = HolKernel.syntax_fns {n = n, dest = d, make = m} "bir_lifting_machines"
 
 fun syntax_fns0 s = let val (tm, _, _, is_f) = syntax_fns 0
@@ -73,18 +73,20 @@ end handle e => raise wrap_exn "dest_bir_lifting_machine_rec" e;
 
 
 (* Array fields *)
+val (bmr_field_extra_tm,  mk_bmr_field_extra, dest_bmr_field_extra, is_bmr_field_extra) =
+ syntax_fns2 (mkselnm "bir_lifting_machine_rec_t" "bmr_extra");
 
-val (bmr_field_extra_tm,  mk_bmr_field_extra, dest_bmr_field_extra, is_bmr_field_extra)  = syntax_fns2 "bir_lifting_machine_rec_t_bmr_extra";
+val (bmr_field_imms_tm,  mk_bmr_field_imms, dest_bmr_field_imms, is_bmr_field_imms) =
+ syntax_fns1 (mkselnm "bir_lifting_machine_rec_t" "bmr_imms");
 
-val (bmr_field_imms_tm,  mk_bmr_field_imms, dest_bmr_field_imms, is_bmr_field_imms)  = syntax_fns1 "bir_lifting_machine_rec_t_bmr_imms";
+val (bmr_field_pc_tm,  mk_bmr_field_pc, dest_bmr_field_pc, is_bmr_field_pc) =
+ syntax_fns1 (mkselnm "bir_lifting_machine_rec_t" "bmr_pc");
 
-val (bmr_field_pc_tm,  mk_bmr_field_pc, dest_bmr_field_pc, is_bmr_field_pc)  = syntax_fns1 "bir_lifting_machine_rec_t_bmr_pc";
+val (bmr_field_mem_tm,  mk_bmr_field_mem, dest_bmr_field_mem, is_bmr_field_mem) =
+ syntax_fns1 (mkselnm "bir_lifting_machine_rec_t" "bmr_mem");
 
-val (bmr_field_mem_tm,  mk_bmr_field_mem, dest_bmr_field_mem, is_bmr_field_mem)  = syntax_fns1 "bir_lifting_machine_rec_t_bmr_mem";
-
-val (bmr_field_step_fun_tm,  mk_bmr_field_step_fun, dest_bmr_field_step_fun, is_bmr_field_step_fun)  = syntax_fns2 "bir_lifting_machine_rec_t_bmr_step_fun";
-
-
+val (bmr_field_step_fun_tm,  mk_bmr_field_step_fun, dest_bmr_field_step_fun, is_bmr_field_step_fun) =
+ syntax_fns2 (mkselnm "bir_lifting_machine_rec_t" "bmr_step_fun");
 (* the main part of bir_lifting_machinesTheory is the record
    type bir_lifting_machine_rec_t. To work with it and related types,
    some rewrites are needed. *)
